Finally have a plausible proof plan for waitgroup; proving that the
a client using waitgroup as required by the documentation actually
results in all the internal panics being avoided was surprisingly
subtle, but it seems like the plan now is no track to do it. Also added
an abstraction for two w32-s encoded as a w64.

new/golang/theory/struct.v
@@ -121,11 +121,11 @@ Proof.
 Qed.
 
 Class StructFieldsSplit `{!IntoVal V} `{!IntoValTyped V t} {dwf : struct.Wf t}
-                        (l : loc) (v : V) (Psplit : iProp Σ)
+                        (dq : dfrac) (l : loc) (v : V) (Psplit : iProp Σ)
   :=
   {
-    struct_fields_split : l ↦ v ⊢ Psplit ;
-    struct_fields_combine : Psplit ⊢ l ↦ v
+    struct_fields_split : l ↦{dq} v ⊢ Psplit ;
+    struct_fields_combine : Psplit ⊢ l ↦{dq} v
   }.
 
 Theorem struct_fields_acc_update f t V Vf
